further work on Remdups example, nearly done

Remdups_Example.thy
@@ -1,7 +1,8 @@
 theory Remdups_Example
-imports HNR_While "SepLogicTime_RBTreeBasic.RBTree_Impl" DataRefinement
+imports HNR_While "SepLogicTime_RBTreeBasic.RBTree_Impl" DataRefinement 
 begin
 
+hide_const R B
 
 subsection "library for some set implementation"
 
@@ -45,7 +46,7 @@ lemma set_ins_hnr:
   sorry
 
 lemma set_ins_hnr':
-  "hn_refine (rbt_map_assn M p) (rbt_insert x () p) emp rbt_map_assn' (set_ins_SPEC x S)"
+  "hn_refine (rbt_map_assn' S p) (rbt_insert x' () p) emp rbt_map_assn' (set_ins_SPEC x S)"
   sorry
 
 
@@ -63,6 +64,12 @@ lemma set_mem_hnr:
   "hn_refine (rbt_map_assn M p) (rbt_search x p) (rbt_map_assn M p) (pure Id) (\<Down>Y (set_mem_SPEC x S))"
   sorry
 
+definition Y' :: "bool \<Rightarrow> unit option \<Rightarrow> assn" where
+  "Y' b v = \<up>(  v = Some () \<longleftrightarrow> b )"
+ 
+lemma set_mem_hnr':
+  "hn_refine (rbt_map_assn' S p) (rbt_search (x'::nat) p) (rbt_map_assn' S p) Y' ( (set_mem_SPEC x S))"
+  sorry 
 
 
 subsection "remdups"
@@ -77,6 +84,7 @@ definition rd_impl1 :: "nat list \<Rightarrow> (nat list) nrest" where
   "rd_impl1 as = do {
           ys \<leftarrow> RETURNT [];
           S \<leftarrow> set_init_SPEC;
+          zs \<leftarrow> RETURNT as;
           whileT (\<lambda>(xs,ys,S). length xs > 0)
             (\<lambda>(xs,ys,S). do {                          
                           ASSERT (length xs > 0);
@@ -88,9 +96,9 @@ definition rd_impl1 :: "nat list \<Rightarrow> (nat list) nrest" where
                           (if b
   then  RETURNT (xs,ys,S)
   else do { S \<leftarrow> set_ins_SPEC x S;
-            ys \<leftarrow> SPECT [x#ys\<mapsto> 10];
+            ys \<leftarrow> RETURNT (x#ys); (* SPECT [x#ys\<mapsto> 10]; *)
             RETURNT (xs,ys,S)
-  } ) }) (as,ys,S);
+  } ) }) (zs,ys,S);
           RETURNT ys
       }"
 
@@ -126,12 +134,203 @@ lemma add_triv: "\<And>B C x. hn_ctxt (pure Id) x x * B \<Longrightarrow>\<^sub>
   using assn_times_comm entails_pure by fastforce  
 
 lemma hd_entails:
-  "hn_val Id a ab \<Longrightarrow>\<^sub>A hn_val Id (hd a) (hd ab)"
+  "hn_val Id (a::nat list) ab \<Longrightarrow>\<^sub>A hn_ctxt (pure Id) (hd a) (hd ab)"
   unfolding hn_ctxt_def   
   by (metis entails_def entails_pure' pair_in_Id_conv pure_app_eq) 
 
+
+
+lemma zuf: "\<up> True * true =  true"  
+  by (simp add: abel_semigroup.commute assn_ext mult.abel_semigroup_axioms)  
+
+
+lemma [simp]: "h\<Turnstile>\<up>b \<longleftrightarrow> (h\<Turnstile>emp \<and> b)" 
+  using one_assn_rule pure_assn_rule by auto 
+
+lemma hn_refine_hd: " hn_refine (hn_val Id s' s)
+           (ureturn (hd s))
+       (hn_val Id s' s)
+       (pure Id) (RETURNT (hd s'))"
+  unfolding hn_refine_def apply (auto simp: zuf mult.assoc  execute_ureturn pure_def hn_ctxt_def)
+   apply(rule exI[where x=0]) apply (auto simp: zero_enat_def relH_def )      
+    using models_in_range top_assn_rule  
+    by (metis (full_types) mod_false zuf)  
+
+
+lemma hn_refine_tl: " hn_refine (hn_val Id s' s)
+           (ureturn (tl s))
+       (hn_val Id s' s)
+       (pure Id) (RETURNT (tl s'))"
+  unfolding hn_refine_def apply (auto simp: zuf mult.assoc  execute_ureturn pure_def hn_ctxt_def)
+   apply(rule exI[where x=0]) apply (auto simp: zero_enat_def relH_def )      
+    using models_in_range top_assn_rule  
+    by (metis (full_types) mod_false zuf)  
+
+
+lemma hnr_cons_rule: " hn_refine (hn_val Id xs' xs * hn_val Id x' x)
+           (ureturn (x#xs))
+       (hn_val Id xs' xs * hn_val Id x' x)
+       (pure Id) (RETURNT (x'#xs'))"
+  unfolding hn_refine_def apply (auto simp: zuf mult.assoc  execute_ureturn pure_def hn_ctxt_def)
+   apply(rule exI[where x=0]) apply (auto simp: zero_enat_def relH_def )      
+  using models_in_range top_assn_rule by blast 
+
+lemma hn_refine_less: " hn_refine (hn_val nat_rel s' s * hn_val nat_rel x' x)
+           (ureturn (x < s))
+       (hn_val nat_rel s' s * hn_val nat_rel x' x)
+       (pure bool_rel) (RETURNT (x' < s'))"
+  unfolding hn_refine_def apply (auto simp: zuf mult.assoc  execute_ureturn pure_def hn_ctxt_def)
+   apply(rule exI[where x=0]) apply (auto simp: zero_enat_def relH_def )      
+    using models_in_range top_assn_rule by blast 
+
+
+lemma manual1: "
+  hn_val Id a ab \<Longrightarrow>\<^sub>A hn_val Id a (XX x' x'a (fst s) (fst (snd s)) (snd (snd s))) \<Longrightarrow>
+   XX = (\<lambda>x' x'a ab ac ba. X x' x'a (ab, ac, ba)) \<Longrightarrow>
+hn_val Id a ab \<Longrightarrow>\<^sub>A hn_val Id a (X x' x'a s)" by auto
+
+schematic_goal "f a = f (?X (a,b,c))"
+  by simp
+
+schematic_goal "hn_val Id a ab \<Longrightarrow>\<^sub>A hn_val Id a (?S x' x'a (ab, ac, ba))"
+  apply(rule entails_triv)      done
+
+schematic_goal "\<And>ab ac ba. f ab = f (?S (ab, ac, ba))"
+  apply(rule refl)      oops
+
+lemma rewr: "P (S' a b c) \<Longrightarrow> S' = (\<lambda>a b c. S (a,b,c)) \<Longrightarrow> P (S (a,b,c))"
+  by auto
+
+
+schematic_goal "\<And>ab ac ba. f ab = f (?S (ab, ac, ba))"
+  apply(rule rewr )
+  apply(rule refl) apply sim      oops
+
+schematic_goal "\<And>x x' xa x'a a aa b ab ac ba.
+       RETURNT x \<le> RETURNT [] \<Longrightarrow>
+       RETURNT xa \<le> set_init_SPEC \<Longrightarrow> a \<noteq> [] \<Longrightarrow> length a + length aa \<le> length as \<Longrightarrow> card b \<le> length aa \<Longrightarrow> hn_val Id a ab \<Longrightarrow>\<^sub>A hn_val Id a (?s73 x' x'a (ab, ac, ba))"
+  apply(rule entails_triv)      oops
+
+
+subsection \<open>Product Types\<close>
+text \<open>Some notion for product types is already defined here, as it is used 
+  for currying and uncurrying, which is fundamental for the sepref tool\<close>
+definition prod_assn :: "('a1\<Rightarrow>'c1\<Rightarrow>assn) \<Rightarrow> ('a2\<Rightarrow>'c2\<Rightarrow>assn) 
+  \<Rightarrow> 'a1*'a2 \<Rightarrow> 'c1*'c2 \<Rightarrow> assn" where
+  "prod_assn P1 P2 a c \<equiv> case (a,c) of ((a1,a2),(c1,c2)) \<Rightarrow>
+  P1 a1 c1 * P2 a2 c2"
+
+
+notation prod_assn (infixr "\<times>\<^sub>a" 70)
+  
+lemma prod_assn_pure_conv[simp]: "prod_assn (pure R1) (pure R2) = pure (R1 \<times>\<^sub>r R2)"
+  by (auto simp: pure_def prod_assn_def pure_conj intro!: ext)
+
+lemma prod_assn_pair_conv[simp]: 
+  "prod_assn A B (a1,b1) (a2,b2) = A a1 a2 * B b1 b2"
+  unfolding prod_assn_def by auto
+
+lemma prod_assn_true[simp]: "prod_assn (\<lambda>_ _. true) (\<lambda>_ _. true) = (\<lambda>_ _. true)"
+  by (auto intro!: ext simp: hn_ctxt_def prod_assn_def)
+
+
+lemma prod_assn_ctxt: "prod_assn A1 A2 x y = z \<Longrightarrow> hn_ctxt (prod_assn A1 A2) x y = z"
+  by (simp add: hn_ctxt_def)
+
+lemma hn_case_prod':
+  assumes FR: "\<Gamma>\<Longrightarrow>\<^sub>thn_ctxt (prod_assn P1 P2) p' p * \<Gamma>1"
+  assumes Pair: "\<And>a1 a2 a1' a2'. \<lbrakk>p'=(a1',a2')\<rbrakk> 
+    \<Longrightarrow> hn_refine (hn_ctxt P1 a1' a1 * hn_ctxt P2 a2' a2 * \<Gamma>1 * hn_invalid (prod_assn P1 P2) p' p) (f a1 a2) 
+          (hn_ctxt P1' a1' a1 * hn_ctxt P2' a2' a2 * hn_ctxt XX1 p' p * \<Gamma>1') R (f' a1' a2')"
+  shows "hn_refine \<Gamma> (case_prod f p) (hn_ctxt (prod_assn P1' P2') p' p * \<Gamma>1')
+    R (case_prod (\<lambda>a b. f' a b) p')" (is "?G \<Gamma>")
+    apply1 (rule hn_refine_cons_pre[OF FR])
+    apply1 extract_hnr_invalids
+    apply1 (cases p; cases p'; simp add: prod_assn_pair_conv[THEN prod_assn_ctxt])
+    apply (rule hn_refine_cons[OF _ Pair _ entt_refl])
+  subgoal
+    apply (simp add: hn_ctxt_def entailst_def)
+          apply(rule ent_true_drop(2))
+          apply(rule ent_true_drop(2)) apply(rule entails_triv) done
+    applyS simp
+      subgoal
+        apply  (simp add: hn_ctxt_def entailst_def mult.assoc)
+    apply(rule match_first)
+    apply(rule match_first) apply(rotatel)
+    apply(rule match_first)  by simp
+      done
+
+    term "pure (Id) \<times>\<^sub>a  pure (Id) \<times>\<^sub>a  rbt_map_assn'"
+  (* nat list \<times> nat list \<times> nat set \<Rightarrow> ?'a23 \<Rightarrow> assn *)
+
+lemma hn_ctxt_prod_split: "hn_ctxt (A \<times>\<^sub>a B) (a, b) (a', b') = hn_ctxt A a a' * hn_ctxt B b b'"
+  by (simp add: prod_assn_def hn_ctxt_def)
+
+lemma hn_ctxt_prod_split': "hn_ctxt (A \<times>\<^sub>a B) (a, b) s' = hn_ctxt A a (fst s') * hn_ctxt B b (snd s')"
+  by (simp add: prod_assn_def hn_ctxt_def  case_prod_beta')  
+
+lemma hn_ctxt_prod_split'': "s'=(a',b') \<Longrightarrow> hn_ctxt (A \<times>\<^sub>a B) (a, b) s' = hn_ctxt A a a' * hn_ctxt B b b'"
+  by (simp add: prod_assn_def hn_ctxt_def  case_prod_beta')  
+
+lemma t: "true = true * true"  
+  by simp  
+
+lemma or_merge: "((B1 * C1) \<or>\<^sub>A (B1 * C2)) = (B1) * (C1 \<or>\<^sub>A C2)"
+  apply(rule ent_iffI)
+  subgoal  by (simp add: ent_disjE match_first) 
+  subgoal sledgehammer sorry
+  oops
+lemma "A * ((B1 * C1) \<or>\<^sub>A (B1 * C2)) = (A * B1) * (C1 \<or>\<^sub>A C2)"
+  apply (simp add: assn_times_assoc or_merge)
+  oops
+
+lemma or_merge: "((B1 * C1) \<or>\<^sub>A (B1 * C2)) \<Longrightarrow>\<^sub>A (B1) * (C1 \<or>\<^sub>A C2)" 
+  by (simp add: ent_disjE match_first) 
+
+lemma or_merge_succ_step: "A * ((B1 * C1) \<or>\<^sub>A (B1 * C2)) \<Longrightarrow>\<^sub>A gr A B1 * (C1 \<or>\<^sub>A C2)"
+  apply (simp add: assn_times_assoc gr_def )
+  apply(rule match_first) using or_merge by auto
+
+lemma or_merge_rotatel: "A * ((B1 * C1) \<or>\<^sub>A (B2 * C2)) \<Longrightarrow>\<^sub>A A * ((C1 * B1) \<or>\<^sub>A (B2 * C2))"
+  apply(rule match_first)  
+  by (simp add: assn_times_comm entails_triv)
+lemma or_merge_rotater: "A * ((B1 * C1) \<or>\<^sub>A (B2 * C2)) \<Longrightarrow>\<^sub>A A * ((B1 * C1) \<or>\<^sub>A (C2 * B2))"
+  apply(rule match_first)  
+  by (simp add: assn_times_comm entails_triv)
+ 
+lemma addemp_triv: "emp * A \<Longrightarrow>\<^sub>A B \<Longrightarrow> A \<Longrightarrow>\<^sub>A B"
+  by simp 
+
+lemma invalid_pure_recover: "invalid_assn (pure R) x y = pure R x y * true"
+  apply (rule ent_iffI) 
+  subgoal
+    apply (rule entailsI)
+    unfolding invalid_assn_def
+    by (auto simp: pure_def assn_times_comm) 
+  subgoal
+    unfolding invalid_assn_def
+    apply (auto simp: pure_def) 
+    using entailsI entails_frame by fastforce 
+  done    
+
+lemma hn_invalid_prod_split: "hn_invalid (A \<times>\<^sub>a B) (a, b) (a', b')
+      \<Longrightarrow>\<^sub>A hn_invalid A a a' * hn_invalid B b b'" 
+  apply(auto simp: hn_ctxt_def invalid_assn_def  )
+  by (smt SepLogic_Misc.mod_pure_star_dist entails_def merge_true_star mod_starD mult.left_commute mult_commute_abs) 
+
+lemma forward_ent: "A \<Longrightarrow>\<^sub>A A' \<Longrightarrow> A' * B \<Longrightarrow>\<^sub>A C \<Longrightarrow> A * B \<Longrightarrow>\<^sub>A C"
+  using entails_frame' by blast 
+
+lemma forward_ent_snd: "B \<Longrightarrow>\<^sub>A B' \<Longrightarrow> A * B' \<Longrightarrow>\<^sub>A C \<Longrightarrow> A * B \<Longrightarrow>\<^sub>A C"
+  sorry
+ 
+lemma underA: "A \<Longrightarrow>\<^sub>A A' \<Longrightarrow> A \<or>\<^sub>A B \<Longrightarrow>\<^sub>A A' \<or>\<^sub>A B"
+  sorry
+
+   
+
 schematic_goal rd_hnr:
- "hn_refine emp ?C ?G ?R (rd_impl1 as)"
+ "hn_refine emp ?C ?G ?R (rd_impl1 as)" using [[goals_limit = 1]]
   unfolding rd_impl1_def
   apply(rule hnr_bind)
     apply(rule hnr_uRETURN_pure[where R=Id]) 
@@ -145,36 +344,211 @@ schematic_goal rd_hnr:
 
   
   apply(rule hnr_bind)
+      apply(rule hnr_frame[OF hnr_uRETURN_pure[where R=Id]]) apply simp
+  apply(simp) apply(rule entt_refl)
 
-  unfolding whileT_I' WHILEIT_to_monadic     
-      apply(rule hn_monadic_WHILE_aux[where Rs="\<lambda>(c1,c2,c3) (a1,a2,a3). (pure Id) c1 a1 * (pure Id) c2 a2 * rbt_map_assn' c3 a3"])
+
+  apply(rule hnr_bind)
+
+  unfolding whileT_I' unfolding WHILEIT_to_monadic     
+(*      apply(rule hn_monadic_WHILE_aux[where Rs="\<lambda>(c1,c2,c3) (a1,a2,a3). (pure Id) c1 a1 * (pure Id) c2 a2 * rbt_map_assn' c3 a3"])
   unfolding entailst_def
           apply rotatel apply(rule match_first)
           apply(rule ent_true_drop(2))
           apply rotatel apply(rule add_triv[where x=as]) 
           apply(rule hn_ctxt_triple')
   unfolding hn_ctxt_triple''
-
-         defer
-
-  apply simp apply(rule match_rest) apply simp
-
-        apply(auto simp del: nres_bind_left_identity) [1]
-  (* the loop body *)
-
-  apply(rule hnr_ASSERT)
-  apply(rule hnr_ASSERT)
-        apply(rule hnr_ASSERT)
-  apply(rule hnr_bind)
-
-          apply(rule hnr_frame[OF hnr_uRETURN_pass])   
-  apply(simp add: entailst_def)
+ *) 
+     apply(rule hn_monadic_WHILE_aux[where Rs="pure (Id) \<times>\<^sub>a  (pure (Id) \<times>\<^sub>a  rbt_map_assn')"])
+  unfolding entailst_def apply(simp  )
+           apply(rule ent_true_drop(2)) apply(rotater)
           apply(rule ent_true_drop(2))
+           apply(subst hn_ctxt_prod_split'') prefer 2
+            apply(subst hn_ctxt_prod_split'') prefer 2
+             apply rotater apply(rule match_first)  apply(rule match_first)  apply(rule entails_triv) apply simp
+           apply simp
+    (* loop guard *)
+  defer 
+  apply(rule match_rest) apply simp
+
+   (* the loop body *)
+   apply(rule hn_case_prod')        
+    apply(simp add: entailst_def  )
+          apply rotatel apply(rule match_first) apply(rule match_rest) apply simp
+
+         apply(rule hn_refine_cons_post'[OF hn_case_prod'])
+           apply(simp add: entailst_def  )
+           apply rotatel  apply (rule match_first)
+  apply rotater apply (rule match_first) apply (rule entails_triv) 
+         
+  apply(rule hnr_ASSERT)
+  apply(rule hnr_ASSERT)
+          apply(rule hnr_ASSERT) 
+  (* the hd operation *)
+  apply(rule hnr_bind[where Rh="pure Id"]) 
+          apply(rule hnr_frame[OF hn_refine_hd])   
+            apply(simp add: entailst_def) apply rotatel apply rotatel apply rotatel apply rotater apply (rule match_first)
+  apply rotater 
+            apply(rule ent_true_drop(2)) apply (rule entails_triv)
+  (* the tl operation *)
+  apply(rule hnr_bind[where Rh="pure Id"]) 
+          apply(rule hnr_frame[OF hn_refine_tl])   
+             apply(simp add: entailst_def mult.assoc) apply rotater apply rotatel apply rotatel    apply rotatel  apply rotatel
+                apply (rule match_first)
+  apply rotater 
+            apply(rule ent_true_drop(2)) apply (rule entails_triv)
+  (* the \<in> operation *)
+  apply(rule hnr_bind )              
+  apply(rule hnr_frame)
+               apply(rule set_mem_hnr') 
+  apply(simp add: entailst_def)
+            apply(rule ent_true_drop(2)) 
+              apply rotater   apply rotatel apply rotatel apply rotatel
+              apply(rule isolate_first) apply(simp add: hn_ctxt_def) apply(rule entails_triv)
+              apply (rule entails_triv)
+
+  (* the if Block *)
+             apply(rule hnr_If')
+                apply rotater apply rotatel apply rotatel apply rotatel apply rotatel apply rotatel apply rotatel apply rotatel
+                apply(rule isolate_first)
+  apply(simp add: hn_ctxt_def Y'_def pure_def   )    
+                 apply(rule entails_triv) 
+  apply rotater 
+            apply(rule ent_true_drop(2)) 
+                apply (rule entails_triv)
+
+  (* 1st if-branch (element already in list ) *)
+               apply(rule hnr_frame) 
+                apply(rule hnr_uRETURN_pass)
+
+  
+               apply(simp add: entailst_def)
+  apply rotater apply rotatel apply rotatel apply swapl apply swapl
+  apply swapl apply swapl  apply swapl apply swapl  
+               apply swapl apply swapl  apply swapl apply takel apply takel 
+  apply(rule isolate_first)
+                apply(simp add:  gr_def     ) 
+                apply(subst hn_ctxt_prod_split'') prefer 2
+  apply(simp add: mult.assoc)
+  apply(rule match_first)
+                apply(subst hn_ctxt_prod_split'') prefer 2
+  apply(rule match_first) apply(simp add: hn_ctxt_def) apply(rule entails_triv)
+  apply simp apply simp
+  apply rotater 
+            apply(rule ent_true_drop(2)) 
+                apply (rule entails_triv)
+
+  (* 2nd if-branch (element should be added ) *)
+
+  apply (rule hnr_bind)
+  (* \<rightarrow> add element into Set *)
+  apply (rule hnr_frame)
+  apply(rule set_ins_hnr')
+                apply(simp add: entailst_def)
+            apply(rule ent_true_drop(2)) 
+                apply rotater apply rotatel apply rotatel apply rotatel apply rotatel apply rotatel apply rotatel
+  apply(rule match_first) 
+                apply (rule entails_triv)
+
+               apply (rule hnr_bind)
+  (* \<rightarrow> append element *)
+
+  apply (simp)
+  apply (rule hnr_frame)
+  apply(rule hnr_cons_rule)
+                apply(simp add: entailst_def)
+            apply(rule ent_true_drop(2)) 
+                 apply rotater apply taker apply rotatel apply rotatel apply rotatel
+                 apply rotatel apply swapl apply takel apply (rule isolate_first)
+                  apply(simp add: gr_def) apply rotatel apply (rule match_first)
+                  apply (rule entails_triv) apply(rule entails_triv)
+
+  (* \<rightarrow> return result *)
+  apply (rule hnr_frame)
+                 apply(rule hnr_uRETURN_pass)
+
+               apply(simp add: entailst_def)
+            apply(rule ent_true_drop(2)) 
+                apply rotater apply rotatel apply rotatel apply rotatel apply rotatel
+                apply swapl apply swapl apply swapl apply takel apply takel
+                apply (rule isolate_first)
+  apply(simp only: gr_def)
+                apply(subst hn_ctxt_prod_split'') prefer 2
+  apply(simp add: mult.assoc)
+  apply(rule match_first)
+                apply(subst hn_ctxt_prod_split'') prefer 2
+  apply(rule match_first) apply(simp add: hn_ctxt_def) apply(rule entails_triv)
+  apply simp apply simp
+                apply (rule entails_triv)
+               apply rotatel apply rotatel apply rotatel apply rotatel apply rotatel apply rotatel
+               apply rotater apply(simp add: mult.assoc) 
+  apply(rule forward_ent[OF hn_invalid_prod_split]) apply rotatel
+               apply(rule forward_ent[OF hn_invalid_prod_split])
+
+  apply(simp add: mult.assoc)
+               apply(rule match_first)
+  apply rotater                         
+            apply(rule ent_true_drop(2)) 
+               apply(rule entails_triv)
+
+            apply(rule ent_true_drop(2)) 
+  apply rotater               
+               apply(rule match_first) 
+               apply(rule entails_triv)      
+
+            apply(rule ent_true_drop(2)) 
+             apply(rule entails_triv)
+
+  (* merge the heap or *)
+  apply(simp only: mult.assoc)
+            apply(rule addemp_triv)
+            apply(rule ent_trans[OF or_merge_succ_step]) 
+            apply(rule ent_trans[OF or_merge_succ_step]) 
+            apply(rule ent_trans[OF or_merge_succ_step]) 
+            apply(rule ent_trans[OF or_merge_rotatel]) 
+  apply(simp only: mult.assoc)
+            apply(rule ent_trans[OF or_merge_succ_step]) 
+            apply(rule ent_trans[OF or_merge_rotatel]) 
+            apply(rule ent_trans[OF or_merge_rotater]) 
+  apply(simp only: mult.assoc)
+            apply(rule ent_trans[OF or_merge_succ_step]) 
+    (* too lazy here to do the rest *)
+
+  (* TODO: recover xd *)
+            apply(rule forward_ent_snd)
+             apply(rule ent_trans) apply(rule underA[OF hn_invalid_prod_split])
+
+
+  apply(simp only: mult.assoc)
+             apply(rule addemp_triv)
+            apply(rule ent_trans[OF or_merge_succ_step])
+            apply(rule forward_ent_snd)
+             apply(rule ent_trans) apply(rule underA[OF hn_invalid_prod_split])
+              apply(simp add: hn_ctxt_def invalid_pure_recover)
+  apply(rule or_merge)
+    
+
+            apply rotater
+  apply(simp add: gr_def mult.assoc)
+            apply(rule isolate_first)
+             apply(simp add: hn_ctxt_def pure_def) apply(rule entails_triv)
   apply rotater
-          apply(rule isolate_first)
-  using hd_entails
-  apply(rule hd_entails)
+            apply(rule ent_true_drop(2))
+            apply(rule entails_triv)
+
+  (* after *)
+   (* recover xd *) defer
+    
+
+               apply taker
+               apply(rule isolate_first)
+  apply(simp only: hn_ctxt_def gr_def invalid_pure_recover)
+                apply(rule match_first) apply simp
+                apply (rule entails_triv)
+              apply(simp add: mult.assoc)
+  apply rotater 
 
 
+  using hnr_cons_rule
 
 end
